resolve admits in traverse; maintenance

templates/lockfree/maintenanceOp_insert.v
@@ -25,29 +25,66 @@ Module MAINTENANCEOP_INSERT.
             ∗ ⌜xs ≡ₚ seq 1 (L-1)⌝ }}}.
 
   Parameter getHeight_spec : ∀ (n: Node) (i: nat),
-    ⊢ <<< ∀∀ h mark next k, node n h mark next k >>>
-          getHeight #n @⊤
-      <<< node n h mark next k, RET #h >>>.
+    ⊢ <<{ ∀∀ h mark next k, node n h mark next k }>>
+          getHeight #n @ ∅
+      <<{ node n h mark next k | RET #h }>>.
 
   Parameter changeNext_spec : ∀ (n m m': Node) (i: nat),
-    ⊢  <<< ∀∀ h mark next k, node n h mark next k ∗ ⌜i < h⌝ >>>
-            changeNext #n #m #m' #i @⊤
-      <<< ∃∃ (success: bool) next',
+    ⊢  <<{ ∀∀ h mark next k, node n h mark next k ∗ ⌜i < h⌝ }>>
+            changeNext #n #m #m' #i @ ∅
+      <<{ ∃∃ (success: bool) next',
               node n h mark next' k
             ∗ (match success with true => ⌜next !! i = Some m 
                                             ∧ mark !!! i = false
                                             ∧ next' = <[i := m']> next⌝
                                 | false => ⌜(next !! i ≠ Some m ∨ 
                                               mark !!! i = true)
-                                            ∧ next' = next⌝ end),
+                                            ∧ next' = next⌝ end) |
               RET (match success with true => SOMEV #() 
-                                    | false => NONEV end)  >>>.
+                                    | false => NONEV end) }>>.
 
-  Lemma maintenanceOp_insert_rec_spec N γ_t γ_s γ_m γ_td1 γ_td2 γ_ght k (n: Node) 
+  Definition traversal_inv γ_m t0 i k p c : iProp :=
+    (∃ s, past_state γ_m t0 s ∗ ⌜p ∈ FP s ∧ Key s p < k ∧ 
+      Marki s p 0 = false ∧ i < Height s p ∧ (i = 0 → Nexti s p i = Some c)⌝)
+  ∗ (∃ s, past_state γ_m t0 s ∗ ⌜c ∈ FP s ∧ i < Height s c⌝).
+
+  Lemma traverse_rec_spec N γ_t γ_r γ_m γ_mt γ_msy tid 
+    t0 k preds succs ps0 ss0 (i: nat):
+    main_inv N γ_t γ_r γ_m γ_mt γ_msy  -∗
+    thread_start γ_t γ_mt tid t0 -∗
+    □ update_helping_protocol2 N γ_t γ_r γ_mt γ_msy -∗ 
+    ⌜1 < L ∧ 0 < k < W⌝ -∗
+      {{{ is_array preds ps0 ∗ is_array succs ss0
+          ∗ ⌜length ps0 = L⌝ ∗ ⌜length ss0 = L⌝ ∗ ⌜i+1 < L⌝
+          ∗ ⌜ps0 !!! (L-1) = hd⌝ ∗ ⌜ss0 !!! (L-1) = tl⌝
+          ∗ (∀ j, ⌜i < j < L⌝ → traversal_inv γ_m t0 j k (ps0 !!! j) (ss0 !!! j)) }}}
+        traverse_rec #k #preds #succs #i @ ⊤
+      {{{ (ps ss: list Node) (res: bool), 
+            RET (#preds, #succs, #res);
+            is_array preds ps ∗ is_array succs ss
+          ∗ ⌜length ps = L⌝ ∗ ⌜length ss = L⌝
+          ∗ ⌜ps !!! (L-1) = hd⌝ ∗ ⌜ss !!! (L-1) = tl⌝
+          ∗ (∀ i, ⌜i < L⌝ → traversal_inv γ_m t0 i k (ps !!! i) (ss !!! i))
+          ∗ (let c := ss !!! 0 in 
+                ∃ s, past_state γ_m t0 s ∗
+                    ⌜if res then 
+                      k ∈ abs s ∧ k = Key s c ∧ c ∈ FP s ∧ Marki s c 0 = false
+                    else 
+                      k ∉ abs s ∧ k < Key s c ∧ c ∈ FP s⌝) }}}.
+  Proof.
+  Admitted.
+
+  Lemma maintenanceOp_insert_rec_spec N γ_t γ_r γ_m γ_mt γ_msy tid t0 k (n: Node) 
     preds succs (ps ss: list Node) perm vs xs (h i: nat):
-    main_inv N γ_t γ_s γ_m γ_td1 γ_td2 γ_ght -∗
+    main_inv N γ_t γ_r γ_m γ_mt γ_msy -∗
+    thread_start γ_t γ_mt tid t0 -∗
+    □ update_helping_protocol2 N γ_t γ_r γ_mt γ_msy -∗ 
+    ⌜1 < L ∧ 0 < k < W⌝ -∗
       {{{   preds ↦∗ ((λ n0 : loc, #n0) <$> ps)
           ∗ succs ↦∗ ((λ n0 : loc, #n0) <$> ss)
+          ∗ ⌜length ps = L⌝ ∗ ⌜length ss = L⌝ ∗ ⌜h < L⌝
+          ∗ ⌜ps !!! (L - 1) = hd⌝ ∗ ⌜ss !!! (L - 1) = tl⌝
+          ∗ (∀ i, ⌜i < L⌝ → traversal_inv γ_m t0 i k (ps !!! i) (ss !!! i))
           ∗ perm ↦∗ vs
           ∗ ⌜vs = (fun n => # (LitInt (Z.of_nat n))) <$> xs⌝
           ∗ ⌜xs ≡ₚ seq 1 (h-1)⌝ }}}
@@ -58,8 +95,10 @@ Module MAINTENANCEOP_INSERT.
           ∗ succs ↦∗ ((λ n0 : loc, #n0) <$> ss')
           ∗ perm ↦∗ vs }}}.
   Proof.
-    iIntros "#HInv". iIntros (Φ) "!# Hpre Hpost".
-    iDestruct "Hpre" as "(Hpreds & Hsuccs & Hperm & %Def_vs & %Perm_xs)".
+    iIntros "#HInv #Thd_st #Upd [%HL %Range_k]". iLöb as "IH" forall (i ps ss). 
+    iIntros (Φ) "!# Hpre Hpost".
+    iDestruct "Hpre" as "(Hpreds & Hsuccs & %Len_ps & %Len_ss & %HhL 
+      & %HpsL & %HssL & #Htr & Hperm & %Def_vs & %Perm_xs)".
     wp_lam. wp_pures. 
     destruct (bool_decide (Z.lt i (h - 1)%Z)) eqn: Hbool; wp_pures.
     - rewrite bool_decide_eq_true in Hbool.
@@ -71,78 +110,282 @@ Module MAINTENANCEOP_INSERT.
       { rewrite Def_vs. rewrite list_lookup_fmap. rewrite Hidx.
         by simpl. }
       iIntros "Hperm". wp_pures.
+      assert (0 < idx < L-1) as HidxL.
+      { apply elem_of_list_lookup_2 in Hidx. rewrite Perm_xs in Hidx.
+        rewrite elem_of_seq in Hidx. lia. }
       assert (is_Some (ps !! idx)) as [p Hp].
-      { admit. }
+      { rewrite lookup_lt_is_Some Len_ps. lia. }
       wp_apply (wp_load_offset _ _ _ (DfracOwn 1) (idx) _ #p
         with "[Hpreds]"); try done.
       { by rewrite list_lookup_fmap Hp /=. }
       iIntros "Hpreds". wp_pures.
       assert (is_Some (ss !! idx)) as [c Hc].
-      { admit. }
+      { rewrite lookup_lt_is_Some Len_ss. lia. }
       wp_apply (wp_load_offset _ _ _ (DfracOwn 1) (idx) _ #c
         with "[Hsuccs]"); try done.
       { by rewrite list_lookup_fmap Hc /=. }
       iIntros "Hsuccs". wp_pures.
       awp_apply changeNext_spec; try done.
       iInv "HInv" as (M0 T0 s0) "(>Ds & >%Habs0 & >Hist & Help & >Templ)".
-      { admit. }
       iDestruct "Templ" as "(SShot0 & Res & %PT0 & %Trans_M0)".
       iDestruct "Res" as "(GKS & Nodes & Nodes_KS)".
+      iAssert (traversal_inv γ_m t0 idx k p c) as "#Htr'".
+      { apply list_lookup_total_correct in Hp. 
+        apply list_lookup_total_correct in Hc.
+        rewrite -Hp -Hc. iApply "Htr". iPureIntro. lia. }
       iAssert (⌜p ∈ FP s0⌝)%I as %FP_p0.
-      { (* interpolation *) admit. }
+      { apply leibniz_equiv in Habs0. rewrite -Habs0.
+        iDestruct "Htr'" as "(Htr'&_)". 
+        iDestruct "Htr'" as (s)"(Past_s & % & _)".
+        iApply (in_FP_2 with "[%] [$Hist] [$Past_s] [%]"); try done.  }
       rewrite (big_sepS_delete _ (FP s0) p); last by eauto.
       iDestruct "Nodes" as "(Node_p & Nodes_rest)".
+      iAssert (⌜idx < Height s0 p⌝)%I as %Height_p0.
+      { apply leibniz_equiv in Habs0. rewrite -Habs0.
+        iDestruct "Htr'" as "(H'&_)". iDestruct "H'" as (s)"(Past_s & %Htr_sc)".
+        destruct Htr_sc as (H'&_&_&H''&_).
+        iPoseProof (height_eq_2 p with "[%] [$Hist] [$Past_s] [%]") as "->"; 
+          try done. }
       iAssert ((node p (Height s0 p) (Mark s0 p) (Next s0 p) (Key s0 p)) 
         ∗ ⌜idx < Height s0 p⌝)%I with "[Node_p]" as "Hpre".
-      { admit. }
+      { iFrame "∗%". }
       iAaccIntro with "Hpre".
       { iIntros "(Node_p & _)". iModIntro. iFrame "Hpost Hperm Hpreds Hsuccs".
         iNext; iExists M0, T0, s0. iFrame "∗%#". 
         rewrite (big_sepS_delete _ (FP s0) p); last by eauto. iFrame. }
       iIntros (success next')"(Node_p & Hif)".
-      destruct success; last first.
+      destruct success; last first; 
+        last destruct (decide (n = c)) as [<- | n_neq_c].
       + iDestruct "Hif" as %[H' ->]. 
         iModIntro. iSplitR "Hpost Hperm Hpreds Hsuccs".
         { iNext. iExists M0, T0, s0. iFrame "∗%".
           rewrite (big_sepS_delete _ (FP s0) p); last by eauto. iFrame. }
-        wp_pures. admit.
-      + admit.
+        wp_pures. 
+        wp_apply (traverse_rec_spec with "[] [] [] [] [Hpreds Hsuccs]"); 
+          try done.
+        { iSplitL "Hpreds". admit. iSplitL "Hsuccs". admit.
+          iSplitL. iPureIntro. apply Len_ps.
+          iSplitL. iPureIntro. apply Len_ss.
+          iSplitL. iPureIntro. lia. iSplitL. by iPureIntro. 
+          iSplitL. by iPureIntro. iIntros (j)"%Hj".
+          assert (j = L-1) as -> by lia. rewrite HpsL HssL. admit. }
+        iIntros (ps' ss' b) "(Hpreds & Hsuccs & %Lep_ps' & %Len_ss' 
+          & %HpsL' & %HssL' & #Htr'' & _)". wp_pures.
+        iSpecialize ("IH" $! i ps' ss').
+        iApply ("IH" with "[-Hpost]"); try done. iFrame "Hperm Htr'' %". admit.
+      + iDestruct "Hif" as %[Next_p0 [Mark_p0 Def_next']].
+        assert (next' = Next s0 p) as Hnext'. 
+        { rewrite Def_next'. apply map_eq. intros i'. 
+          destruct (decide (i' = idx)) as [-> | Hi]. 
+          by rewrite lookup_insert Next_p0. by rewrite lookup_insert_ne. }
+        rewrite Hnext'.
+        iModIntro. iSplitR "Hpost Hperm Hsuccs Hpreds".
+        { iNext. iExists M0, T0, s0. iFrame "∗#%".
+          rewrite (big_sepS_delete _ (FP s0) p); try done. iFrame. }
+        wp_pures. iSpecialize ("IH" $! (i+1) ps ss).
+        assert (Z.add i 1 = (i+1)%nat) as ->. clear; lia.
+        iApply ("IH" with "[-Hpost]"); try done. 
+        { iSplitL "Hpreds". admit. iSplitL "Hsuccs". admit. 
+          iSplitR. iPureIntro. apply Len_ps.
+          iSplitR. iPureIntro. apply Len_ss.
+          iSplitR. iPureIntro. lia. iSplitR. by iPureIntro. 
+          iSplitR. by iPureIntro. iFrame "Htr". iFrame "Hperm".
+          by iPureIntro. }
+      + iDestruct "Hif" as %[Next_p0 [Mark_p0 Def_next']].
+        iDestruct "SShot0" as %[FP0 [C0 [Ht0 [Mk0 [Nx0 [Ky0 [I0 
+            [Hs0 [Dom_Ht0 [Dom_Mk0 [Dom_Nx0 [Dom_Ky0 Dom_I0]]]]]]]]]]]].
+        set Nx0' := <[p := next']> Nx0.
+        set s0' := (FP0, C0, Ht0, Mk0, Nx0', Ky0, I0): snapshot.
+        set M0' := <[T0 + 1 := s0']> M0.
+        
+        iAssert (⌜per_tick_inv s0⌝)%I as %PT_s0.
+        { iApply (per_tick_current with "[%] [%] [$Hist]"); try done. }
+
+        assert (FP s0' = FP s0) as FP_s0'.
+        { by rewrite /FP /s0' Hs0. }
+        assert (abs s0' = abs s0) as Habs'.
+        { by rewrite /abs /s0' Hs0. }
+        iAssert (dsRepI γ_r (abs s0'))%I with "[Ds]" as "Ds".
+        { by rewrite Habs'. }
+        iAssert (own γ_ks (● prodKS (KS, abs s0')))%I with "[GKS]" as "GKS".
+        { by rewrite Habs'. }
+        assert (∀ n, n ≠ p → Next s0' n = Next s0 n) as HN.
+        { intros n' Hnp. 
+          rewrite /Next /s0' Hs0 /= /Nx0' lookup_insert_ne; try done. }
+        assert (Next s0' p = <[idx:=n]> (Next s0 p)) as HNp.
+        { by rewrite /s0' Hs0 /Next /Nx0' lookup_insert Def_next' /Next Hs0. }
+        assert (∀ n, Key s0' n = Key s0 n) as HK.
+        { by rewrite /Key /s0' Hs0 /=. }
+        assert (∀ n, FI s0' n = FI s0 n) as HI.
+        { by rewrite /FI /s0' Hs0 /=. }
+        assert (∀ n, Mark s0' n = Mark s0 n) as HM.
+        { by rewrite /FI /s0' Hs0. }
+        assert (∀ n, Height s0' n = Height s0 n) as HT.
+        { by rewrite /FI /s0' Hs0. }
+
+        iAssert (⌜snapshot_constraints s0'⌝)%I as "SShot1'".
+        { iPureIntro. exists FP0, C0, Ht0, Mk0, Nx0', Ky0, I0.
+          repeat split; try done.
+          rewrite /Nx0'. rewrite dom_insert_L.
+          assert (p ∈ dom Nx0). 
+          { rewrite Hs0 in FP_p0. rewrite Dom_Nx0. by unfold FP in FP_p0. }
+          clear -H Dom_Nx0. set_solver. }
+
+        iAssert (resources γ_ks s0')%I 
+          with "[GKS Nodes_KS Node_p Nodes_rest]" as "Res".
+        { iFrame "GKS". rewrite FP_s0'. iSplitR "Nodes_KS".
+          rewrite (big_opS_delete _ (FP s0) p); try done.
+          iSplitL "Node_p". rewrite Def_next' HNp HT HM HK. done.
+          iApply (big_sepS_mono with "Nodes_rest"); try done.
+          intros x Hx. iIntros "Hn". rewrite HK HT HM HN. done.
+          clear -Hx; set_solver.
+          iApply (big_sepS_mono with "Nodes_KS"); try done.
+          intros x Hx. iIntros "Hn". rewrite HI.
+          assert (Content s0' x = Content s0 x) as ->.
+          rewrite /Content HK /Marki HM. done. done. }
+        
+        assert (p ≠ tl) as p_neq_tl. admit.
+        assert (n ∈ FP s0) as FP_n0. admit.
+        assert (idx < Height s0 n) as Hidxn. admit.
+        
+        assert (per_tick_inv s0') as PT_s0'.
+        { destruct PT_s0 as (PT1'&PT2'&PT3'&PT4'&PT5'&PT6'&PT7').
+          split; last split; last split; last split; last split; last split.
+          - rewrite FP_s0' !HK !HM !HT. repeat split; try apply PT1'. 
+            destruct (decide (p = hd)) as [-> | Hphd]. 
+            rewrite HNp. rewrite lookup_insert_ne. apply PT1'. clear -HidxL; lia.
+            all: rewrite HN; try done; apply PT1'.
+          - rewrite /s0' /GFI /FP /FI. by rewrite Hs0 /GFI /FP /FI in PT2'.
+          - intros n' k'. rewrite FP_s0' HI Habs' /Content /Marki HM HK.
+            apply PT3'.
+          - intros n' Hn. rewrite FP_s0' in Hn. apply PT4' in Hn.
+            destruct (decide (n' = p)) as [-> | Hnp].
+            + rewrite HNp HK HI HT HM.
+              destruct Hn as (Hn1&Hn2&Hn3&Hn4&Hn5&Hn6).
+              split; last split; last split; last split; last split; try done.
+              * intros H'. assert (H1' := H'). apply Hn2 in H1'. 
+                rewrite dom_insert_L H1'.
+                assert (idx ∈ gset_seq 0 (Height s0 p - 1)) as H''.
+                rewrite elem_of_gset_seq. split; try lia.
+                clear -H''; set_solver.
+              * rewrite lookup_insert_ne; try done. lia.
+            + rewrite HK HT HI HM. rewrite HN; try done.
+          - intros n1 n2. destruct (decide (n1 = p)) as [-> | Hn1p].
+            + rewrite /Nexti HNp !HK. 
+              rewrite lookup_insert_ne; try done. apply PT5'. lia.
+            + rewrite !HK /Nexti HN; try done. apply PT5'. 
+          - intros n1 n2 i'. rewrite FP_s0'. 
+            destruct (decide (n1 = p)) as [-> | Hn1p].
+            + rewrite /Nexti HNp. destruct (decide (i' = idx)) as [-> | Hi'i].
+              rewrite lookup_insert. intros [=<-]. done. 
+              rewrite lookup_insert_ne; try done. apply PT6'.
+            + rewrite /Nexti HN; try done. apply PT6'.
+          - intros n1 n2 i'. rewrite /Nexti. 
+            destruct (decide (n1 = p)) as [-> | Hn1p]; last first.
+            { rewrite HT HN; try done. apply PT7'. }
+            rewrite HNp. destruct (decide (i' = idx)) as [-> | Hii'].
+            + rewrite lookup_insert HT. intros [=<-]. done.
+            + rewrite HT lookup_insert_ne; try done. apply PT7'. }
+        assert (transition_inv s0 s0') as Trans_s0.
+        { repeat split; try rewrite FP_s0'; try done; last first.
+          - intros n' i' Hfp. rewrite /Marki HM. done.
+          - intros n'. rewrite /Marki HM. intros H' H''. 
+            rewrite H' in H''; try done.
+          - intros n' i' Hn'. destruct (decide (n' = p)) as [-> | Hnp].
+            + rewrite /Marki HM /Nexti HNp. 
+              destruct (decide (i' = idx)) as [-> | Hi].
+              rewrite Mark_p0. clear; try done.
+              rewrite lookup_insert_ne; try done.
+            + rewrite /Marki /Nexti HM HN; try done. }
+
+        iAssert (⌜dom M0 = gset_seq 0 T0⌝)%I as %Dom_M0. 
+        { by iDestruct "Hist" as (M0'') "(_&_&%&_)". }
+              
+        iAssert (|==> hist γ_t γ_m M0' (T0+1))%I with "[Hist]" as ">Hist".
+        { iPoseProof (hist_upd _ _ _ _ _ s0' with "[%] [%] [$Hist]") as ">H'".
+          apply  Habs0. intros <-. rewrite map_eq_iff in HNp.
+          pose proof HNp idx as HNp. rewrite Next_p0 lookup_insert in HNp.
+          inversion HNp; try done. by rewrite /M0'. }
+        iAssert (helping_inv N γ_t γ_r γ_mt γ_msy M0')%I with
+          "[Help]" as "Help".
+        { unfold update_helping_protocol2.
+          iSpecialize ("Upd" $! M0 T0 s0').
+          iPoseProof ("Upd" with "[%] [%] [Help]") as "Help"; try done.
+          apply leibniz_equiv in Habs0. rewrite Habs0. by rewrite /s0' Hs0 /=.
+          admit. }
+        iModIntro. iSplitR "Hpost Hperm Hpreds Hsuccs".
+        { iNext. iExists M0', (T0+1), s0'. iFrame "∗#%".
+          iPureIntro; rewrite /M0'; split; last split.
+          - by rewrite lookup_total_insert.
+          - intros t Ht. destruct (decide (t = T0+1)) as [-> | Ht'].
+            + by rewrite lookup_total_insert.
+            + rewrite lookup_total_insert_ne; try done. apply PT0.
+              rewrite dom_insert in Ht. clear -Ht' Ht; set_solver.
+          - intros t Ht. destruct (decide (t = T0)) as [-> | Ht'].
+            + rewrite lookup_total_insert. rewrite lookup_total_insert_ne.
+              apply leibniz_equiv in Habs0. by rewrite Habs0. clear; lia.
+            + rewrite !lookup_total_insert_ne. apply Trans_M0.
+              all: clear -Ht Ht'; lia. }
+        wp_pures. iSpecialize ("IH" $! (i+1) ps ss).
+        assert (Z.add i 1 = (i+1)%nat) as ->. clear; lia.
+        iApply ("IH" with "[-Hpost]"); try done. 
+        { iSplitL "Hpreds". admit. iSplitL "Hsuccs". admit. 
+          iSplitR. iPureIntro. apply Len_ps.
+          iSplitR. iPureIntro. apply Len_ss.
+          iSplitR. iPureIntro. lia. iSplitR. by iPureIntro. 
+          iSplitR. by iPureIntro. iFrame "Htr". iFrame "Hperm".
+          by iPureIntro. }
   Admitted.
 
-  Lemma maintenanceOp_insert_spec N γ_t γ_s γ_m γ_td1 γ_td2 γ_ght k (n:Node) preds succs 
-    ps ss:
-      main_inv N γ_t γ_s γ_m γ_td1 γ_td2 γ_ght -∗
+  Lemma maintenanceOp_insert_spec N γ_t γ_r γ_m γ_mt γ_msy tid t0 k (n:Node) 
+    preds succs ps ss:
+    main_inv N γ_t γ_r γ_m γ_mt γ_msy -∗
+    thread_start γ_t γ_mt tid t0 -∗
+    □ update_helping_protocol2 N γ_t γ_r γ_mt γ_msy -∗ 
+    ⌜1 < L ∧ 0 < k < W⌝ -∗
         {{{   preds ↦∗ ((λ n0 : loc, #n0) <$> ps)
-            ∗ succs ↦∗ ((λ n0 : loc, #n0) <$> ss) }}}
+            ∗ succs ↦∗ ((λ n0 : loc, #n0) <$> ss)
+            ∗ (∃ s, past_state γ_m t0 s ∗ ⌜n ∈ FP s⌝)
+            ∗ ⌜length ps = L⌝ ∗ ⌜length ss = L⌝
+            ∗ ⌜ps !!! (L - 1) = hd⌝ ∗ ⌜ss !!! (L - 1) = tl⌝
+            ∗ (∀ i, ⌜i < L⌝ → traversal_inv γ_m t0 i k (ps !!! i) (ss !!! i)) }}}
            maintenanceOp_insert #k #preds #succs #n
         {{{ (ps' ss': list Node),
             RET #();
               preds ↦∗ ((λ n0 : loc, #n0) <$> ps')
             ∗ succs ↦∗ ((λ n0 : loc, #n0) <$> ss') }}}.
   Proof.
-    iIntros "#HInv". iIntros (Φ) "!# (Hpreds & Hsuccs) Hpost".
+    iIntros "#HInv #Thd_st #Upd [%HL %Range_k]". 
+    iIntros (Φ) "!# (Hpreds&Hsuccs&#FP_n&%Len_ps&%Len_ss&%HpsL&%HssL&#Htr) Hpost".
     wp_lam. wp_pures. awp_apply getHeight_spec; try done.
-    { admit. }
     iInv "HInv" as (M0 T0 s0) "(>Ds & >%Habs0 & >Hist & Help & >Templ)".
-    { admit. }
     iDestruct "Templ" as "(SShot0 & Res & %PT0 & %Trans_M0)".
     iDestruct "Res" as "(GKS & Nodes & Nodes_KS)".
     iAssert (⌜n ∈ FP s0⌝)%I as %FP_n0.
-    { (* interpolation *) admit. }
+    { apply leibniz_equiv in Habs0. rewrite -Habs0.
+      iDestruct "FP_n" as (s)"(Past_s & %)".
+      iApply (in_FP_2 with "[%] [$Hist] [$Past_s] [%]"); try done. }
     rewrite (big_sepS_delete _ (FP s0) n); last by eauto.
     iDestruct "Nodes" as "(Node_n & Nodes_rest)".
     iAaccIntro with "Node_n".
     { iIntros "Node_n". iModIntro. iFrame.
       iNext; iExists M0, T0, s0. iFrame "∗%#". 
       rewrite (big_sepS_delete _ (FP s0) n); try done. iFrame. }
-    iIntros "Node_n". iSplitR "Hpreds Hsuccs Hpost".
+    iIntros "Node_n". 
+    set h := Height s0 n. 
+    iAssert (⌜per_tick_inv s0⌝)%I as %PT_s0.
+    { iApply (per_tick_current with "[%] [%] [$Hist]"); try done. }
+    assert (h < L). 
+    { apply PT_s0 in FP_n0. destruct FP_n0 as (_&_&_&H'&_). admit. }
+    iSplitR "Hpreds Hsuccs Hpost".
     { iModIntro. iNext; iExists M0, T0, s0. iFrame "∗%#". 
-      rewrite (big_sepS_delete _ (FP s0) n); try done. iFrame. }  
-    iModIntro. wp_pures. set h := Height s0 n. 
+      rewrite (big_sepS_delete _ (FP s0) n); try done. iFrame. } 
+    iModIntro. wp_pures. 
     wp_apply permute_levels_spec; try done.
     iIntros (perm vs xs)"(Hperm & %Def_vs & %Perm_xs)". wp_pures. 
-    wp_apply (maintenanceOp_insert_rec_spec with "[] [$Hperm $Hpreds $Hsuccs]"); 
-      try done.
+    wp_apply (maintenanceOp_insert_rec_spec with "[] [] [] [] 
+      [$Hperm $Hpreds $Hsuccs]"); try done.
+    { iFrame "#%". }
     iIntros (ps' ss')"(Hpreds & Hsuccs & Hperm)". 
     iApply "Hpost". iFrame.
   Admitted.
