templates/lockfree/maintenanceOp_delete.v
@@ -17,21 +17,21 @@ Module MAINTENANCEOP_DELETE.
   Import SKIPLIST1 SKIPLIST1_UTIL.DEFS SKIPLIST1_UTIL.
 
   Parameter markNode_spec : ∀ (n: Node) (i: nat),
-    ⊢  <<< ∀∀ h mark next k, node n h mark next k ∗ ⌜i < h⌝ >>>
-            markNode #n #i @⊤
-      <<< ∃∃ (success: bool) mark',
+    ⊢  <<{ ∀∀ h mark next k, node n h mark next k ∗ ⌜i < h⌝ }>>
+            markNode #n #i @ ∅
+      <<{ ∃∃ (success: bool) mark',
               node n h mark' next k
             ∗ (match success with true => ⌜mark !!! i = false
                                             ∧ mark' = <[i := true]> mark⌝
                                 | false => ⌜mark !!! i = true
-                                            ∧ mark' = mark⌝ end),
+                                            ∧ mark' = mark⌝ end) |
               RET (match success with true => SOMEV #() 
-                                    | false => NONEV end)  >>>.
+                                    | false => NONEV end) }>>.
 
   Parameter getHeight_spec : ∀ (n: Node) (i: nat),
-    ⊢ <<< ∀∀ h mark next k, node n h mark next k >>>
-          getHeight #n @⊤
-      <<< node n h mark next k, RET #h >>>.
+    ⊢ <<{ ∀∀ h mark next k, node n h mark next k }>>
+          getHeight #n @ ∅
+      <<{ node n h mark next k | RET #h }>>.
 
   Parameter permute_levels_spec : ∀ (L: nat),
         {{{ True }}}
@@ -41,22 +41,24 @@ Module MAINTENANCEOP_DELETE.
             ∗ ⌜vs = (fun n => # (LitInt (Z.of_nat n))) <$> xs⌝
             ∗ ⌜xs ≡ₚ seq 1 (L-1)⌝ }}}.
 
-  Lemma maintenanceOp_delete_rec_spec N γ_t γ_s γ_m γ_td1 γ_td2 γ_ght t0 c
+  Lemma maintenanceOp_delete_rec_spec N γ_t γ_r γ_m γ_mt γ_msy tid t0 c
     perm vs xs i h:
-      main_inv N γ_t γ_s γ_m γ_td1 γ_td2 γ_ght -∗
+    main_inv N γ_t γ_r γ_m γ_mt γ_msy  -∗
+    thread_start γ_t γ_mt tid t0 -∗
+    □ update_helping_protocol2 N γ_t γ_r γ_mt γ_msy -∗ 
         {{{   perm ↦∗ vs
             ∗ ⌜vs = (fun n => # (LitInt (Z.of_nat n))) <$> xs⌝
             ∗ ⌜xs ≡ₚ seq 1 (h-1)⌝
             ∗ (∃ s, past_state γ_m t0 s ∗ ⌜c ∈ FP s⌝ ∗ ⌜h = Height s c⌝
                     ∗ ⌜∀ j, j < i → Marki s c (xs !!! j) = true⌝)
             ∗ ⌜c ≠ hd⌝ ∗ ⌜c ≠ tl⌝ }}}
-           maintenanceOp_delete_rec #i #h #perm #c
+           maintenanceOp_delete_rec #i #h #perm #c @ ⊤
         {{{ RET #();
               (∃ s, past_state γ_m t0 s ∗ ⌜c ∈ FP s⌝ ∗ ⌜h = Height s c⌝
                     ∗ ⌜∀ j, j < h-1 → Marki s c (xs !!! j) = true⌝)
             ∗ perm ↦∗ vs }}}.
   Proof.
-    iIntros "#HInv". iLöb as "IH" forall (i).
+    iIntros "#HInv #Thd_st #Upd". iLöb as "IH" forall (i).
     iIntros (Φ) "!# (Hperm&%Def_vs&%Perm_xs&#Hmark&%c_neq_hd&%c_neq_tl) Hpost". 
     wp_lam. wp_pures.
     destruct (bool_decide (Z.lt i (h - 1)%Z)) eqn: Hbool; wp_pures.
@@ -71,7 +73,6 @@ Module MAINTENANCEOP_DELETE.
       iIntros "Hperm". wp_pures.
       awp_apply markNode_spec; try done.
       iInv "HInv" as (M0 T0 s0) "(>Ds & >%Habs0 & >Hist & Help & >Templ)".
-      { admit. }
       iDestruct "Templ" as "(SShot0 & Res & %PT0 & %Trans_M0)".
       iDestruct "Res" as "(GKS & Nodes & Nodes_KS)".
       iAssert (⌜c ∈ FP s0⌝)%I as %FP_c0.
@@ -102,6 +103,13 @@ Module MAINTENANCEOP_DELETE.
         apply Hj' in Hj. apply leibniz_equiv in Habs0. rewrite -Habs0.
         iPoseProof (marking_mono_2 c with "[%] [$Hist] [$Past_s] [%]") as "->"; 
             try done. }
+      iAssert (⌜dom M0 = gset_seq 0 T0⌝)%I as %Dom_M0. 
+      { by iDestruct "Hist" as (M0'') "(_&_&%&_)". }
+      iAssert (own γ_t (◯ MaxNat t0)) as "#Ht0".
+      { iDestruct "Thd_st" as "(_&H')". iFrame "H'". }      
+      iPoseProof (snapshot_current with "[%] [$Ht0] [$Hist]") 
+        as ">(#Past_s0&Hist)"; try done.
+
       iIntros (success mark')"(Node_c & Hif)". destruct success.
       + iDestruct "Hif" as %[Mark_c0 Def_mark'].
         iDestruct "SShot0" as %[FP0 [C0 [Ht0 [Mk0 [Nx0 [Ky0 [I0 
@@ -110,41 +118,12 @@ Module MAINTENANCEOP_DELETE.
         set s0' := (FP0, C0, Ht0, Mk0', Nx0, Ky0, I0): snapshot.
         set M0' := <[T0 + 1 := s0']> M0.
         iAssert (⌜per_tick_inv s0⌝)%I as %PT_s0.
-        { iDestruct "Hist" as (M')"(_&_&_&%&_)". iPureIntro.
-          apply leibniz_equiv in Habs0. rewrite <-Habs0.
-          by apply PT0. }
-        iAssert (hist γ_t γ_m M0' (T0+1))%I with "[Hist]" as "Hist".
-        { admit. }
-        iAssert (▷ helping_inv N γ_t γ_s γ_td1 γ_td2 γ_ght M0')%I with
-          "[Help]" as "Help".
-        { admit. }
-        iAssert (past_state γ_m t0 s0')%I as "Past_s0'".
-        { admit. } 
-        iAssert (∃ s : snapshot, past_state γ_m t0 s ∗ ⌜c ∈ FP s⌝ ∗ ⌜h = Height s c⌝
-          ∗ ⌜∀ j : nat, j < i + 1 → Marki s c (xs !!! j) = true⌝)%I as "#Hmark'".
-        { iDestruct "Hmark" as (s) "(Hpast_s & %FP_c' & %Ht_c & %Hj)".
-          iAssert (⌜Marki s0' c (xs !!! i) = true⌝)%I as %Hi.
-          { iPureIntro. rewrite list_lookup_total_alt Hidx /=.
-            rewrite /s0' /Marki /Mark /Mk0' lookup_insert Def_mark'.
-            by rewrite lookup_total_insert. }
-          iExists s0'. iFrame "Past_s0'". iPureIntro.
-          split. rewrite /s0' /FP. by rewrite Hs0 /FP in FP_c0.
-          split. rewrite /s0' /Height. rewrite Hs0 /Height in Ht_c0. done.
-          intros j Hj'. destruct (decide (j = i)) as [-> | Hji]; try done.
-          rewrite /s0' /Marki /Mark /Mk0' lookup_insert Def_mark'.
-          rewrite lookup_total_insert_ne. rewrite /Marki in Hj0.
-          apply Hj0. lia. 
-          clear -Hji Hj' Hidx Hbool Perm_xs. intros H'. apply Hji.
-          assert (is_Some (xs !! j)) as [idx' Hidx'].
-          apply lookup_lt_is_Some. rewrite Perm_xs seq_length. lia.
-          assert (idx' = idx) as ->. by rewrite H' list_lookup_total_alt Hidx' /=. 
-          assert (NoDup xs) as H''. rewrite Perm_xs. apply NoDup_seq.
-          by pose proof NoDup_lookup xs i j idx H'' Hidx Hidx'. }
+        { iApply (per_tick_current with "[%] [%] [$Hist]"); try done. }
         assert (FP s0' = FP s0) as FP_s0'.
         { by rewrite /FP /s0' Hs0. }
         assert (abs s0' = abs s0) as Habs'.
         { by rewrite /abs /s0' Hs0. }
-        iAssert (dsRepI γ_s (abs s0'))%I with "[Ds]" as "Ds".
+        iAssert (dsRepI γ_r (abs s0'))%I with "[Ds]" as "Ds".
         { by rewrite Habs'. }
         iAssert (own γ_ks (● prodKS (KS, abs s0')))%I with "[GKS]" as "GKS".
         { by rewrite Habs'. }
@@ -174,11 +153,16 @@ Module MAINTENANCEOP_DELETE.
           { rewrite Hs0 in FP_c0. rewrite Dom_Mk0. by unfold FP in FP_c0. }
           clear -H Dom_Mk0. set_solver. }
         assert (per_tick_inv s0') as PT_s0'.
-        { destruct PT_s0 as (PT1&PT2&PT3&PT4&PT5&PT6).
-          split; last split; last split; last split; last split.
+        { destruct PT_s0 as (PT1&PT2&PT3&PT4&PT5&PT6&PT7).
+          split; last split; last split; last split; last split; last split.
           - rewrite FP_s0' !HK !HN !HT !HM; try done.
           - rewrite /s0' /GFI /FP /FI. by rewrite Hs0 /GFI /FP /FI in PT2.
-          - intros n Hn. rewrite FP_s0' in Hn. apply PT3 in Hn.
+          - intros n k. rewrite FP_s0' HI Habs' /Content /Marki HK.
+            destruct (decide (n = c)) as [-> | Hnc].
+            + rewrite HMc lookup_total_insert_ne; try done.
+              apply PT3.
+            + rewrite HM; try done. apply PT3.
+          - intros n Hn. rewrite FP_s0' in Hn. apply PT4 in Hn.
             destruct (decide (n = c)) as [-> | Hnc].
             + rewrite HT HN HK HI HMc.
               destruct Hn as (Hn1&Hn2&Hn3&Hn4&Hn5&Hn6).
@@ -194,9 +178,9 @@ Module MAINTENANCEOP_DELETE.
                 clear -H'; set_solver.
               * rewrite lookup_total_insert_ne; try done.
             + rewrite HT HN HK HI HM; try done.
-          - intros n1 n2. rewrite /Nexti. rewrite HN !HK. apply PT4.
-          - intros n1 n2 i'. rewrite /Nexti. rewrite HN FP_s0'. apply PT5.
-          - intros n1 n2 i'. rewrite /Nexti HT HN. apply PT6. }
+          - intros n1 n2. rewrite /Nexti. rewrite HN !HK. apply PT5.
+          - intros n1 n2 i'. rewrite /Nexti. rewrite HN FP_s0'. apply PT6.
+          - intros n1 n2 i'. rewrite /Nexti HT HN. apply PT7. }
         assert (transition_inv s0 s0') as Trans_s0.
         { repeat split; try rewrite FP_s0'; try done; last first.
           intros n i' Hn; rewrite /Marki; intros Hm.
@@ -225,6 +209,43 @@ Module MAINTENANCEOP_DELETE.
           rewrite /Content HK. destruct (decide (x = c)) as [-> | Hxc].
           rewrite /Marki HMc lookup_total_insert_ne; try done.
           rewrite /Marki HM; try done. done. }
+        iAssert (|==> hist γ_t γ_m M0' (T0+1))%I with "[Hist]" as ">Hist".
+        { iPoseProof (hist_upd _ _ _ _ _ s0' with "[%] [%] [$Hist]") as ">H'".
+          apply Habs0. intros <-. rewrite map_eq_iff in HMc.
+          pose proof HMc idx as HMc. rewrite lookup_insert in HMc.
+          apply lookup_total_correct in HMc. by rewrite Mark_c0 in HMc.
+          by rewrite /M0'. }
+        iAssert (helping_inv N γ_t γ_r γ_mt γ_msy M0')%I with
+          "[Help]" as "Help".
+        { unfold update_helping_protocol2.
+          iSpecialize ("Upd" $! M0 T0 s0').
+          iPoseProof ("Upd" with "[%] [%] [Help]") as "Help"; try done.
+          apply leibniz_equiv in Habs0. rewrite Habs0. by rewrite /s0' Hs0 /=.
+          admit. }
+        iPoseProof (snapshot_current with "[%] [$Ht0] [$Hist]") 
+          as ">(#Past_s0'&Hist)"; try done.
+        iEval (rewrite /M0' lookup_total_insert) in "Past_s0'".
+        iAssert (∃ s : snapshot, past_state γ_m t0 s ∗ ⌜c ∈ FP s⌝ ∗ ⌜h = Height s c⌝
+          ∗ ⌜∀ j : nat, j < i + 1 → Marki s c (xs !!! j) = true⌝)%I as "#Hmark'".
+        { iDestruct "Hmark" as (s) "(Hpast_s & %FP_c' & %Ht_c & %Hj)".
+          iAssert (⌜Marki s0' c (xs !!! i) = true⌝)%I as %Hi.
+          { iPureIntro. rewrite list_lookup_total_alt Hidx /=.
+            rewrite /s0' /Marki /Mark /Mk0' lookup_insert Def_mark'.
+            by rewrite lookup_total_insert. }
+          iExists s0'. iFrame "Past_s0'". iPureIntro.
+          split. rewrite /s0' /FP. by rewrite Hs0 /FP in FP_c0.
+          split. rewrite /s0' /Height. rewrite Hs0 /Height in Ht_c0. done.
+          intros j Hj'. destruct (decide (j = i)) as [-> | Hji]; try done.
+          rewrite /s0' /Marki /Mark /Mk0' lookup_insert Def_mark'.
+          rewrite lookup_total_insert_ne. rewrite /Marki in Hj0.
+          apply Hj0. lia. 
+          clear -Hji Hj' Hidx Hbool Perm_xs. intros H'. apply Hji.
+          assert (is_Some (xs !! j)) as [idx' Hidx'].
+          apply lookup_lt_is_Some. rewrite Perm_xs seq_length. lia.
+          assert (idx' = idx) as ->. by rewrite H' list_lookup_total_alt Hidx' /=. 
+          assert (NoDup xs) as H''. rewrite Perm_xs. apply NoDup_seq.
+          by pose proof NoDup_lookup xs i j idx H'' Hidx Hidx'. }
+
         iModIntro. iSplitR "Hperm Hpost".
         { iNext. iExists M0', (T0+1), s0'. iFrame "∗#%".
           iPureIntro; rewrite /M0'; split; last split.
@@ -248,7 +269,7 @@ Module MAINTENANCEOP_DELETE.
           ∗ ⌜∀ j : nat, j < i + 1 → Marki s c (xs !!! j) = true⌝)%I as "#Hmark'".
         { iAssert (⌜Marki s0 c (xs !!! i) = true⌝)%I as %Hi.
           { iPureIntro. rewrite list_lookup_total_alt Hidx /=. done. }
-          iExists s0. iSplitL. iExists T0. admit.
+          iExists s0. iFrame "Past_s0". 
           iPureIntro; split; try done. split. done.
           intros j Hj. destruct (decide (j = i)) as [-> | Hji]; try done.
           apply Hj0. lia. }
@@ -269,18 +290,19 @@ Module MAINTENANCEOP_DELETE.
   Admitted.
 
     
-  Lemma maintenanceOp_delete_spec N γ_t γ_s γ_m γ_td1 γ_td2 γ_ght t0 c:
-      main_inv N γ_t γ_s γ_m γ_td1 γ_td2 γ_ght -∗
-        {{{ (∃ s, past_state γ_m t0 s ∗ ⌜c ∈ FP s⌝) ∗ ⌜c ≠ hd⌝ ∗ ⌜c ≠ tl⌝ }}}
-           maintenanceOp_delete #c
+  Lemma maintenanceOp_delete_spec N γ_t γ_r γ_m γ_mt γ_msy tid t0 c:
+    main_inv N γ_t γ_r γ_m γ_mt γ_msy  -∗
+    thread_start γ_t γ_mt tid t0 -∗
+    □ update_helping_protocol2 N γ_t γ_r γ_mt γ_msy -∗ 
+      {{{ (∃ s, past_state γ_m t0 s ∗ ⌜c ∈ FP s⌝) ∗ ⌜c ≠ hd⌝ ∗ ⌜c ≠ tl⌝ }}}
+           maintenanceOp_delete #c @ ⊤
         {{{ RET #();
               (∃ s h, past_state γ_m t0 s ∗ ⌜c ∈ FP s⌝ ∗ ⌜h = Height s c⌝
                     ∗ ⌜∀ i, 1 ≤ i < h → Marki s c i = true⌝) }}}.
   Proof.
-    iIntros "#HInv". iIntros (Φ) "!# (#FP_c & %c_neq_hd & %c_neq_tl) Hpost".
+    iIntros "#HInv #Thd_st #Upd". iIntros (Φ) "!# (#FP_c&%c_neq_hd&%c_neq_tl) Hpost".
     wp_lam. wp_pures. awp_apply getHeight_spec; try done. 
     iInv "HInv" as (M0 T0 s0) "(>Ds & >%Habs0 & >Hist & Help & >Templ)".
-    { admit. }
     iDestruct "Templ" as "(SShot0 & Res & %PT0 & %Trans_M0)".
     iDestruct "Res" as "(GKS & Nodes & Nodes_KS)".
     iAssert (⌜c ∈ FP s0⌝)%I as %FP_c0.
@@ -294,14 +316,18 @@ Module MAINTENANCEOP_DELETE.
       iNext; iExists M0, T0, s0. iFrame "∗%#". 
       rewrite (big_sepS_delete _ (FP s0) c); try done. iFrame. }
     iIntros "Node_c". 
+    iAssert (own γ_t (◯ MaxNat t0)) as "#Ht0".
+    { iDestruct "Thd_st" as "(_&H')". iFrame "H'". }      
+    iPoseProof (snapshot_current with "[%] [$Ht0] [$Hist]") 
+      as ">(#Past_s0&Hist)"; try done.
     iSplitR " Hpost".
     { iModIntro. iNext; iExists M0, T0, s0. iFrame "∗%#". 
       rewrite (big_sepS_delete _ (FP s0) c); try done. iFrame. }  
     iModIntro. wp_pures. set h := Height s0 c. 
     wp_apply permute_levels_spec; try done.
     iIntros (perm vs xs)"(Hperm & %Def_vs & %Perm_xs)". wp_pures. 
-    wp_apply (maintenanceOp_delete_rec_spec with "[] [Hperm]"); try done.
-    { iFrame "Hperm %". iExists s0. iSplitL. admit. 
+    wp_apply (maintenanceOp_delete_rec_spec with "[] [] [] [Hperm]"); try done.
+    { iFrame "Hperm %". iExists s0. iFrame "Past_s0".
       iPureIntro. repeat split; try done. lia. }
     iIntros "(Hs & Hperm)". iDestruct "Hs" as (s)"(Hs & %H' & %H'' & %H1')".
     iApply "Hpost". iExists s, h; iFrame. iPureIntro; repeat split; try done.
@@ -312,6 +338,6 @@ Module MAINTENANCEOP_DELETE.
       by rewrite Perm_xs seq_length in Hjxs. 
       by rewrite list_lookup_total_alt Hjxs. }
     apply H1'; try done.
-  Admitted.
+  Qed.
 
 End MAINTENANCEOP_DELETE.
